Isabelle/AList_ext.thy
@@ -17,7 +17,7 @@ by (simp add: is_alist_def)
 lemma alist_subset_is_alist: "is_alist (x # l) \<Longrightarrow> is_alist l"
 by (induct l) (auto simp add: is_alist_def)
 
-lemma key_in_fst: "(k, v) \<in> A \<Longrightarrow> k \<in> fst ` A"
+lemma key_in_fst[simp]: "(k, v) \<in> A \<Longrightarrow> k \<in> fst ` A"
 by (rule Set.image_eqI) simp_all
 
 lemma key_filter_empty: "(k \<notin> fst ` set l) = ([(ka, v)\<leftarrow>l . ka = k] = [])"
@@ -31,12 +31,12 @@ by (simp add: of_key_def restrict_single)
 
 lemma existence_from_of_key: "is_alist l \<Longrightarrow> k \<in> fst ` set l \<Longrightarrow> of_key l k = v \<Longrightarrow> (k, v) \<in> set l"
   unfolding restrict_single
-by (induct l) (auto simp add: of_key_def key_in_fst restrict_eq key_filter_empty is_alist_def)
+by (induct l) (auto simp add: of_key_def restrict_eq key_filter_empty is_alist_def)
 
 lemma of_key_predicate: "is_alist l \<Longrightarrow> (k, v) \<in> set l \<Longrightarrow> P k v \<Longrightarrow> P k (of_key l k)"
-by (induct l) (auto simp add: of_key_def is_alist_def key_in_fst)
+by (induct l) (auto simp add: of_key_def is_alist_def)
 
 lemma of_key_forall: "\<forall>(k, v) \<in> set l. P k v \<Longrightarrow> k \<in> fst ` set l \<Longrightarrow> P k (of_key l k)"
-by (induct l) (auto simp add: of_key_def key_in_fst)
+by (induct l) (auto simp add: of_key_def)
 
 end
